trying to fix the cancellation tactic.

src/ILTac.v
@@ -56,6 +56,7 @@ Section existsSubst.
     end.
 End existsSubst.
 
+(*
 Lemma apply_CancelSep : forall ts,
   let types := Env.repr BedrockCoreEnv.core ts in
   forall (funcs : functions types) (preds : SEP.predicates types BedrockCoreEnv.pc BedrockCoreEnv.st), 
@@ -82,7 +83,7 @@ Lemma apply_CancelSep : forall ts,
         (*SH.liftSHeap 0 (length vars') ( *) SH.sheapSubstU 0 (length qr) (length uvars') rhs (* ) *)
       in
       let post :=
-        {| UNF.Vars  := vars'
+        {| UNF.Vars  := List.app ql (rev (skipn (length ql) (vars')))
          ; UNF.UVars := uvars' ++ rev qr
          ; UNF.Heap  := rhs
          |}
@@ -120,80 +121,217 @@ Proof.
 
   Transparent UNF.backward UNF.forward Env.repr.
 Admitted.
+*)
 
-Lemma ApplyCancelSep : forall ts,
-  let types := Env.repr BedrockCoreEnv.core ts in
-  forall (funcs : functions types) (preds : SEP.predicates types BedrockCoreEnv.pc BedrockCoreEnv.st), 
-  forall (algos : ILAlgoTypes.AllAlgos ts), ILAlgoTypes.AllAlgos_correct funcs preds algos ->
-  let prover := 
-    match ILAlgoTypes.Prover algos with
-      | None => provers.ReflexivityProver.reflexivityProver
-      | Some p => p
-    end
-  in
-  let hints :=
-    match ILAlgoTypes.Hints algos with
-      | None => UNF.default_hintsPayload _ _ _ 
-      | Some h => h
-    end
-  in
-  forall (meta_env : env (Env.repr BedrockCoreEnv.core types)) (hyps : Expr.exprs (_))
-  (l r : SEP.sexpr types BedrockCoreEnv.pc BedrockCoreEnv.st),
-  Expr.AllProvable funcs meta_env nil hyps ->
-  let (ql, lhs) := SH.hash l in
-  let facts := Summarize prover (map (liftExpr 0 0 0 (length ql)) hyps ++ SH.pures lhs) in
-  forall cs,
-  let pre :=
-    {| UNF.Vars  := ql
-     ; UNF.UVars := map (@projT1 _ _) meta_env
-     ; UNF.Heap  := lhs
-     |}
-  in
-  match UNF.forward hints prover 10 facts pre with
-    | {| UNF.Vars := vars' ; UNF.UVars := uvars' ; UNF.Heap := lhs |} =>
-      let (qr, rhs) := SH.hash r in
-      let rhs := 
-        (*SH.liftSHeap 0 (length vars') ( *) SH.sheapSubstU 0 (length qr) (length uvars') rhs (* ) *)
-      in
-      let post :=
-        {| UNF.Vars  := vars'
-         ; UNF.UVars := uvars' ++ rev qr
-         ; UNF.Heap  := rhs
-         |}
-      in
-      match UNF.backward hints prover 10 facts post with
-        | {| UNF.Vars := vars' ; UNF.UVars := uvars' ; UNF.Heap := rhs |} =>
-          let new_vars  := vars' in
-          let new_uvars := skipn (length meta_env) uvars' in
-          let bound := length uvars' in
-          match CANCEL.sepCancel preds prover bound facts lhs rhs with
-            | (lhs', rhs', subst) =>
-              Expr.forallEach (rev new_vars) (fun nvs : Expr.env types =>
-                let var_env := nvs in
-                Expr.AllProvable_impl funcs meta_env var_env
-                  (existsSubst (exprD funcs meta_env var_env) subst 0 
-                    (map (fun x => existT (fun t => option (tvarD types t)) (projT1 x) (Some (projT2 x))) meta_env ++
-                     map (fun x => existT (fun t => option (tvarD types t)) x None) new_uvars)
-                    (fun meta_env : Expr.env types =>
-                      (Expr.AllProvable_and funcs meta_env var_env
-                        (himp cs 
-                          (SEP.sexprD funcs preds meta_env var_env
-                            (SH.sheapD (SH.Build_SHeap _ _ (SH.impures lhs') nil (SH.other lhs'))))
-                          (SEP.sexprD funcs preds meta_env var_env
-                            (SH.sheapD (SH.Build_SHeap _ _ (SH.impures rhs') nil (SH.other rhs')))))
-                        (SH.pures rhs')) ))
-                  (SH.pures lhs'))
-          end
+Section canceller.
+  Variable ts : list type.
+  Let types := Env.repr BedrockCoreEnv.core ts.
+  Variable funcs : functions types.
+  Variable preds : SEP.predicates types BedrockCoreEnv.pc BedrockCoreEnv.st.
+  Variable algos : ILAlgoTypes.AllAlgos ts.
+
+  Record CancellerResult : Type :=
+  { AllExt : variables
+  ; ExExt  : variables
+  ; Lhs    : SH.SHeap types BedrockCoreEnv.pc BedrockCoreEnv.st
+  ; Rhs    : SH.SHeap types BedrockCoreEnv.pc BedrockCoreEnv.st
+  ; Subst  : U.Subst types
+  }.
+  
+  Definition canceller (uvars : list tvar) (hyps : Expr.exprs types)
+    (lhs rhs : SEP.sexpr types BedrockCoreEnv.pc BedrockCoreEnv.st) : CancellerResult :=
+    let prover := 
+      match ILAlgoTypes.Prover algos with
+        | None => provers.ReflexivityProver.reflexivityProver
+        | Some p => p
       end
-  end ->
-  himp cs (@SEP.sexprD _ _ _ funcs preds meta_env nil l)
-          (@SEP.sexprD _ _ _ funcs preds meta_env nil r).
-Proof.
-  Opaque UNF.backward UNF.forward Env.repr.
-  intros; destruct algos; destruct Hints; destruct Prover; eapply apply_CancelSep; eauto; destruct X; eauto; simpl in *;
-  eauto using provers.ReflexivityProver.reflexivityProver_correct, UNF.hintsSoundness_default.
-  Transparent UNF.backward UNF.forward Env.repr.
-Qed.
+    in
+    let hints :=
+      match ILAlgoTypes.Hints algos with
+        | None => UNF.default_hintsPayload _ _ _ 
+        | Some h => h
+      end
+    in
+    let (ql, lhs) := SH.hash lhs in
+    let facts := Summarize prover (map (liftExpr 0 0 0 (length ql)) hyps ++ SH.pures lhs) in
+    let pre :=
+      {| UNF.Vars  := rev ql
+       ; UNF.UVars := uvars
+       ; UNF.Heap  := lhs
+      |}
+    in
+    match UNF.forward hints prover 10 facts pre with
+      | {| UNF.Vars := vars' ; UNF.UVars := uvars' ; UNF.Heap := lhs |} =>
+        let (qr, rhs) := SH.hash rhs in
+        let rhs := 
+          (*SH.liftSHeap 0 (length vars') ( *) SH.sheapSubstU 0 (length qr) (length uvars') rhs (* ) *)
+        in
+        let post :=
+          {| UNF.Vars  := vars' (* List.app ql (rev (skipn (length ql) (vars'))) *)
+           ; UNF.UVars := uvars' ++ rev qr
+           ; UNF.Heap  := rhs
+          |}
+        in
+        match UNF.backward hints prover 10 facts post with
+          | {| UNF.Vars := vars' ; UNF.UVars := uvars' ; UNF.Heap := rhs |} =>
+            let new_vars  := vars' in
+            let new_uvars := skipn (length uvars) uvars' in
+            let bound := length uvars' in
+            match CANCEL.sepCancel preds prover bound facts lhs rhs with
+              | (l,r,s) =>
+                {| AllExt := new_vars
+                 ; ExExt  := new_uvars
+                 ; Lhs    := l
+                 ; Rhs    := r
+                 ; Subst  := s
+                 |}
+            end
+        end
+    end.
+
+  Lemma ApplyCancelSep_with_eq : 
+    forall (algos_correct : ILAlgoTypes.AllAlgos_correct funcs preds algos),
+    forall (meta_env : env (Env.repr BedrockCoreEnv.core types)) (hyps : Expr.exprs (_)),
+    Expr.AllProvable funcs meta_env nil hyps ->
+    forall (l r : SEP.sexpr types BedrockCoreEnv.pc BedrockCoreEnv.st) res cs,
+    forall (WTR : SEP.WellTyped_sexpr (typeof_funcs funcs) (SEP.typeof_preds preds) (typeof_env meta_env) nil r = true),
+    canceller (typeof_env meta_env) hyps l r = res ->
+    match res with
+      | {| AllExt := new_vars
+         ; ExExt  := new_uvars
+         ; Lhs    := lhs'
+         ; Rhs    := rhs'
+         ; Subst  := subst
+         |} =>
+        Expr.forallEach ((*rev*) new_vars) (fun nvs : Expr.env types =>
+          let var_env := nvs in
+          Expr.AllProvable_impl funcs meta_env var_env
+            (existsSubst (exprD funcs meta_env var_env) subst 0 
+              (map (fun x => existT (fun t => option (tvarD types t)) (projT1 x) (Some (projT2 x))) meta_env ++
+               map (fun x => existT (fun t => option (tvarD types t)) x None) new_uvars)
+              (fun meta_env : Expr.env types =>
+                (Expr.AllProvable_and funcs meta_env var_env
+                  (himp cs 
+                    (SEP.sexprD funcs preds meta_env var_env
+                      (SH.sheapD (SH.Build_SHeap _ _ (SH.impures lhs') nil (SH.other lhs'))))
+                    (SEP.sexprD funcs preds meta_env var_env
+                      (SH.sheapD (SH.Build_SHeap _ _ (SH.impures rhs') nil (SH.other rhs')))))
+                  (SH.pures rhs')) ))
+            (SH.pures lhs'))
+    end ->
+    himp cs (@SEP.sexprD _ _ _ funcs preds meta_env nil l)
+            (@SEP.sexprD _ _ _ funcs preds meta_env nil r).
+  Proof.
+    Opaque UNF.backward UNF.forward Env.repr.
+    intros. unfold canceller in *.
+    assert (PC : ProverT_correct
+              match ILAlgoTypes.Prover algos with
+              | Some p => p
+              | None => ReflexivityProver.reflexivityProver
+              end funcs).
+    { generalize (ILAlgoTypes.Acorrect_Prover algos_correct).
+      destruct (ILAlgoTypes.Prover algos); intros; auto.
+      apply ReflexivityProver.reflexivityProver_correct. }
+    generalize dependent (match ILAlgoTypes.Prover algos with
+                            | Some p => p
+                            | None => ReflexivityProver.reflexivityProver
+                          end).
+    match goal with
+      | [ |- context [ ?X ] ] =>
+        match X with 
+          | match ILAlgoTypes.Hints _ with _ => _ end =>
+            assert (HC : UNF.hintsSoundness funcs preds X); [ | generalize dependent X ]
+        end
+    end.
+    { generalize (ILAlgoTypes.Acorrect_Hints algos_correct).     
+      destruct (ILAlgoTypes.Hints algos); auto using UNF.hintsSoundness_default. }
+    intros h HC p ? PC.
+    consider (SH.hash l); intros.
+    rewrite SH.hash_denote. rewrite H0; clear H0; simpl.
+    consider (SH.hash r); intros.
+    rewrite SH.hash_denote with (s := r). rewrite H0; simpl.
+    rewrite UNF.himp_existsEach_ST_EXT_existsEach.
+    rewrite UNF.ST_EXT.himp_existsEach_p; [ reflexivity | intros ].
+    rewrite app_nil_r.
+    assert (AllProvable funcs meta_env (rev G) (SH.pures s)) by admit.
+    match goal with 
+      | [ H : context [ Summarize ?P ?ps ] |- _ ] =>
+        assert (Valid PC meta_env (rev G) (Summarize P ps)); [ | generalize dependent (Summarize P ps); intros ]
+    end.
+    { eapply Summarize_correct.
+      apply AllProvable_app; auto.
+      revert H; clear - H3. induction hyps; simpl; intros; auto.
+      intuition. clear - H0 H3. unfold Provable in *.
+      generalize (liftExpr_ext funcs meta_env nil nil nil (rev G) nil a tvProp); simpl.
+      rewrite app_nil_r. rewrite rev_length. subst. rewrite map_length.
+      intro. rewrite H in *. auto. }
+    match goal with
+      | [ H : match ?X with _ => _ end = _ |- _ ] => consider X
+    end; intros.
+    assert (SH.WellTyped_sheap (typeof_funcs funcs) (UNF.SE.typeof_preds preds)
+      (typeof_env meta_env) (rev v) s = true) by admit.
+    destruct (UNF.forwardLength _ _ _ _ _ H2).
+    eapply UNF.forwardOk  with (cs := cs) in H2; simpl; eauto using typeof_env_WellTyped_env.
+    Focus 2. unfold WellTyped_env. subst. rewrite <- map_rev. auto.
+    rewrite H2; clear H2. simpl.
+    rewrite UNF.ST_EXT.himp_existsEach_p; [ reflexivity | intros ].
+    simpl in *. destruct H8.
+    consider (UNF.backward h p 10 f
+           {| UNF.Vars := Vars
+            ; UNF.UVars := UVars ++ rev v0
+            ; UNF.Heap := SH.sheapSubstU 0 (length v0) (length UVars) s0 |}); intros.
+    destruct (UNF.backwardLength _ _ _ _ _ H6); simpl in *.
+    consider (CANCEL.sepCancel preds p (length UVars0) f Heap Heap0); intros.
+    destruct p0. intuition; subst.
+    eapply forallEach_sem in H1. Focus 2. instantiate (1 := rev G ++ G0).
+    rewrite typeof_env_app. f_equal. rewrite <- map_rev. reflexivity.
+    rewrite ListFacts.rw_skipn_app in H2. apply H2. repeat rewrite rev_length. rewrite map_length. auto.
+    Lemma AllProvable_impl_AllProvable : forall U G P ps,
+      AllProvable funcs U G ps ->
+      AllProvable_impl funcs U G P ps ->
+      P.
+    Proof. clear. induction ps; simpl; intros; eauto. intuition. Qed.
+    eapply AllProvable_impl_AllProvable in H1; [ | admit ]. (** TODO **)
+    
+    Transparent UNF.backward UNF.forward Env.repr.
+  Admitted.
+
+  Lemma ApplyCancelSep : 
+    forall (algos_correct : ILAlgoTypes.AllAlgos_correct funcs preds algos),
+    forall (meta_env : env (Env.repr BedrockCoreEnv.core types)) (hyps : Expr.exprs (_)),
+    Expr.AllProvable funcs meta_env nil hyps ->
+    forall (l r : SEP.sexpr types BedrockCoreEnv.pc BedrockCoreEnv.st) cs,
+    forall (WTR : SEP.WellTyped_sexpr (typeof_funcs funcs) (SEP.typeof_preds preds) (typeof_env meta_env) nil r = true),
+    match canceller (typeof_env meta_env) hyps l r with
+      | {| AllExt := new_vars
+         ; ExExt  := new_uvars
+         ; Lhs    := lhs'
+         ; Rhs    := rhs'
+         ; Subst  := subst
+         |} =>
+        Expr.forallEach ((*rev*) new_vars) (fun nvs : Expr.env types =>
+          let var_env := nvs in
+          Expr.AllProvable_impl funcs meta_env var_env
+            (existsSubst (exprD funcs meta_env var_env) subst 0 
+              (map (fun x => existT (fun t => option (tvarD types t)) (projT1 x) (Some (projT2 x))) meta_env ++
+               map (fun x => existT (fun t => option (tvarD types t)) x None) new_uvars)
+              (fun meta_env : Expr.env types =>
+                (Expr.AllProvable_and funcs meta_env var_env
+                  (himp cs 
+                    (SEP.sexprD funcs preds meta_env var_env
+                      (SH.sheapD (SH.Build_SHeap _ _ (SH.impures lhs') nil (SH.other lhs'))))
+                    (SEP.sexprD funcs preds meta_env var_env
+                      (SH.sheapD (SH.Build_SHeap _ _ (SH.impures rhs') nil (SH.other rhs')))))
+                  (SH.pures rhs')) ))
+            (SH.pures lhs'))
+    end ->
+    himp cs (@SEP.sexprD _ _ _ funcs preds meta_env nil l)
+            (@SEP.sexprD _ _ _ funcs preds meta_env nil r).
+  Proof.
+    intros. eapply ApplyCancelSep_with_eq; eauto.
+  Qed.
+
+End canceller.
 
 Lemma interp_interp_himp : forall cs P Q stn_st,
   interp cs (![ P ] stn_st) ->
@@ -360,7 +498,8 @@ Ltac sep_canceler isConst ext simplifier :=
         (((** TODO: for some reason the partial application to proofs doesn't always work... **)
          apply (@ApplyCancelSep typesV funcsV predsV 
                    (ILAlgoTypes.Algos ext typesV)
-                   (@ILAlgoTypes.Algos_correct ext typesV funcsV predsV) uvars pures L R); [ apply proofs | ]
+                   (@ILAlgoTypes.Algos_correct ext typesV funcsV predsV) uvars pures L R); 
+           [ apply proofs | vm_compute; reflexivity | ]
 (*TIME       ;  stop_timer "sep_canceler:apply_CancelSep" *)
  )
         || (idtac "failed to apply, generalizing instead!" ;
